\chapter{Research Results}

\section{Notation for the AIBP}
\noindent
Let:
\begin{itemize}
  \item $\bm \sigma = (\sigma_1,..\sigma_n)$ of ${1,...n}$ gives the sequence
        in which the n items are allocated, where the $t^{th}$ item allocated
        is $\sigma_t$. 
  \item $\lambda(i,j)$ = similarity between customers $i$ and $j$.
  \item $x_i$ be the number of \textit{new} dishes that customer $i$ draws.\\ 
  \item $y_{-i} = \suml{j}{1}{i-1} x_j$, the number of existing dishes
        before customer $i$ draws new dishes.
  \item $g_i(x_i) = \ds\frac{(\alpha/i)^{x_i}\exp(-\alpha/i)}{x_i!}$, 
        which is the probability mass function for a Poisson distribution 
        with parameter $\alpha/i$ and argument $x_i$.\\
  \item $K$ = the number of non-zero columns in $\bm Z$.\\
  \item $m_{-i,k}$ = the number of customers that took dish $k$ before customer
        customer $i$.
  \item $m_{-i} = \suml{k}{1}{K}m_{-i,k}$.
  \item $h_{i,k} = \ds\frac{\sums{\sigma}{z_{-i,k}=1}{}\lambda(\sigma,\sigma_i)}
        {\suml{k}{1}{y_i}\left(\sums{\sigma}{z_{-i,k}=1}{}\lambda(\sigma,\sigma_i)
         \right)}$
  \item $p_{i,k} = h_{i,k} \ds\frac{m_{-i}}{i}$
  %\item $h(i) = \prodl{k}{1}{y_{-i}} 
  %      (p_{i,k})^{z_{i,k}}(1-p_{i,k})^{1-z_{i,k}}$, for $i>1$,
  %      and $1$ for $i=1$.
  \item $H_N = \suml{i}{1}{N} \ds\frac{1}{i}$.
\end{itemize}


\section{Sampling Algorithm for the AIBP}
\begin{itemize}
  \item The first customer draws an $x_1=$ Poisson($\alpha$) number of dishes. This
        is indicated by setting $z_{1,1:x_1}$ to $1$.
  \item For the next $i$ customers, for $i=1:N$, 
     \begin{itemize}
       \item if there exists previously sampled dishes, then customer $i$
             samples dish k with probability $\left(h_{i,k}\right) 
             \left(\ds\frac{m_{-i}}{i}\right)$, for $ k = 1:y_{-i}$.
       \item customer $i$ draws another Poisson($\alpha/i$) number of new dishes.
     \end{itemize}
\end{itemize}


\section{Probability Mass Function}
\begin{align*}
  \text{P}(\bm Z|\bm\sigma)
  =&\prodl{i}{1}{N} \left\{g_i(x_i) \prodl{k}{1}{y_{-i}} 
    (p_{i,k})^{z_{i,k}}(1-p_{i,k})^{1-z_{i,k}}\right\}\\
  =&\prodl{i}{1}{N} \left\{ \ds\frac{(\alpha/i)^{x_i}\exp(-\alpha/i)}{x_i!} 
    \prodl{k}{1}{y_{-i}} 
    \ds\frac{(h_{i,k}m{-i})^{z_{i,k}}(i-h_{i,k}m_{-i,k})^{1-z_{i,k}}}{i} 
    \right\} \\
  =&\ds\frac{\alpha^{\suml{i}{1}{N}x_i} \exp(-\alpha H_N)} {\prodl{i}{1}{N}x_i!} 
    \left( \prodl{i}{1}{N}i^{-x_i} \right) \times
    \\
    &\left( \prodl{i}{1}{N}\prodl{k}{1}{y_{-i}} 
    \ds\frac{\left(\hik m_{-i}\right)^{z_{i,k}}
             \left(i-\hik m_{-i}\right)^{1-z_{i,k}}}{i} \right)\\
  =&\ds\frac{\alpha^K \exp(-\alpha H_N)} {\prodl{i}{1}{N}x_i!} 
    \left( \prodl{i}{2}{N} i^{-x_i-y_{-i}}\prodl{k}{1}{y_{-i}} 
    \ds\frac{
    \left(\sums{\sigma}{z_{-i,k}=1}{}\lambda(\sigma,\sigma_i)m_{-i}\right)^{z_{i,k}}
    \left(i-\sums{\sigma}{z_{-i,k}=1}{}
    \lambda(\sigma,\sigma_i)m_{-i}\right)^{1-z_{i,k}}
    }
    {\suml{k}{1}{y_{-i}}\sums{\sigma}{z_{-i,k}=1}{}\lambda(\sigma,\sigma_i)}\right)
\end{align*}


\section{Simulation Study}
% Provide link to code of simulation.

\section{Comparisons between the AIBP \& ddIBP}
% Closed form pmf
% E[#columns]
% E[rowsum] all equal
% E[colsum]
% E[cell values]
\begin{center}
  \begin{tabular}{c|c|c}
    \hline
      Comparison & AIBP & ddIBP \\ \hline \hline
      Closed form pmf & Yes & No \\ \hline
      Explicit pmf & Yes & No \\ \hline
      Expected non-zero columns equal to that of IBP & Yes & No \\ \hline
      Expected row sums equal to that of IBP & No & Yes \\ \hline
      Expected column sums equal to that of IBP & No & No \\ \hline
      Expected matrix sum equal to that of IBP & No & Yes \\ \hline
    \hline
  \end{tabular}
\end{center}

